*** empty log message ***

doc-src/TutorialI/Types/Pairs.thy
@@ -1,4 +1,4 @@
-(*<*)theory Pairs imports Main begin(*>*)
+(*<*)theory Pairs imports Main begin hide const swap(*>*)
 
 section{*Pairs and Tuples*}
 
@@ -57,20 +57,20 @@ The most obvious approach is the brute force expansion of @{term split}:
 lemma "(\<lambda>(x,y).x) p = fst p"
 by(simp add: split_def)
 
-text{* This works well if rewriting with @{thm[source]split_def} finishes the
+text{* \noindent
+This works well if rewriting with @{thm[source]split_def} finishes the
 proof, as it does above.  But if it does not, you end up with exactly what
 we are trying to avoid: nests of @{term fst} and @{term snd}. Thus this
 approach is neither elegant nor very practical in large examples, although it
 can be effective in small ones.
 
 If we consider why this lemma presents a problem, 
-we quickly realize that we need to replace the variable~@{term
+we realize that we need to replace variable~@{term
 p} by some pair @{term"(a,b)"}.  Then both sides of the
 equation would simplify to @{term a} by the simplification rules
 @{thm split_conv[no_vars]} and @{thm fst_conv[no_vars]}.  
 To reason about tuple patterns requires some way of
 converting a variable of product type into a pair.
-
 In case of a subterm of the form @{term"split f p"} this is easy: the split
 rule @{thm[source]split_split} replaces @{term p} by a pair:%
 \index{*split (method)}
@@ -126,9 +126,7 @@ may be present in the goal. Consider the following function:
 *}
 
 (*<*)by(simp split: split_split_asm)(*>*)
-consts swap :: "'a \<times> 'b \<Rightarrow> 'b \<times> 'a"
-primrec
-  "swap (x,y) = (y,x)"
+primrec swap :: "'a \<times> 'b \<Rightarrow> 'b \<times> 'a" where "swap (x,y) = (y,x)"
 
 text{*\noindent
 Note that the above \isacommand{primrec} definition is admissible
@@ -138,10 +136,10 @@ because @{text"\<times>"} is a datatype. When we now try to prove
 lemma "swap(swap p) = p"
 
 txt{*\noindent
-simplification will do nothing, because the defining equation for @{const swap}
-expects a pair. Again, we need to turn @{term p} into a pair first, but this
-time there is no @{term split} in sight. In this case the only thing we can do
-is to split the term by hand:
+simplification will do nothing, because the defining equation for
+@{const[source] swap} expects a pair. Again, we need to turn @{term p}
+into a pair first, but this time there is no @{term split} in sight.
+The only thing we can do is to split the term by hand:
 *}
 apply(case_tac p)
 
@@ -154,9 +152,8 @@ Splitting by @{text case_tac} also solves the previous examples and may thus
 appear preferable to the more arcane methods introduced first. However, see
 the warning about @{text case_tac} in \S\ref{sec:struct-ind-case}.
 
-In case the term to be split is a quantified variable, there are more options.
-You can split \emph{all} @{text"\<And>"}-quantified variables in a goal
-with the rewrite rule @{thm[source]split_paired_all}:
+Alternatively, you can split \emph{all} @{text"\<And>"}-quantified variables
+in a goal with the rewrite rule @{thm[source]split_paired_all}:
 *}
 
 (*<*)by simp(*>*)
@@ -164,7 +161,7 @@ lemma "\<And>p q. swap(swap p) = q \<longrightarrow> p = q"
 apply(simp only: split_paired_all)
 
 txt{*\noindent
-@{subgoals[display,indent=0]}
+@{subgoals[display,indent=0,margin=70]}
 *}
 
 apply simp
@@ -195,7 +192,7 @@ lemma "\<forall>p. \<exists>q. swap p = swap q"
 by simp;
 
 text{*\noindent
-To turn off this automatic splitting, just disable the
+To turn off this automatic splitting, disable the
 responsible simplification rules:
 \begin{center}
 @{thm split_paired_All[no_vars]}
